ml-dsa: Spec.Intrinsics: backport more intrinsics from core-models

libcrux-ml-dsa/proofs/fstar/spec/Spec.Intrinsics.fst
@@ -2,18 +2,22 @@ module Spec.Intrinsics
 open Core
 open Core_models.Core_arch.X86.Interpretations.Int_vec
 
+let i32x4 = Core_models.Abstractions.Funarr.t_FunArray (mk_u64 4) i32
+let bv128 = Core_models.Abstractions.Bitvec.t_BitVec (mk_u64 128)
+
 let i32x8 = Core_models.Abstractions.Funarr.t_FunArray (mk_u64 8) i32
 let i64x4 = Core_models.Abstractions.Funarr.t_FunArray (mk_u64 4) i64
 let bv256 = Core_models.Abstractions.Bitvec.t_BitVec (mk_u64 256)
 
 assume val to_i32x8 (x:Core_models.Abstractions.Bitvec.t_BitVec (mk_u64 256)): i32x8
+assume val to_i32x4 (x: bv128): i32x4
 assume val from_i32x8 (x:i32x8): Core_models.Abstractions.Bitvec.t_BitVec (mk_u64 256)
 assume val to_from_i32x8_lemma (x:i32x8):
   Lemma (to_i32x8 (from_i32x8 x) == x) [SMTPat (to_i32x8 (from_i32x8 x))]
 
 let mm256_shuffle_epi32_index (a:i32) (i:u64{v i<4}) : u64 =
   cast ((a >>! (i *! mk_u64 2 <: u64) <: i32) %! mk_i32 4 <: i32) <: u64
-  
+
 assume val mm256_shuffle_epi32_lemma (a:i32) (b:bv256) (i:u64{v i < 8}):
   Lemma (to_i32x8 (Libcrux_intrinsics.Avx2.mm256_shuffle_epi32 a b) i ==
        (if i <. mk_u64 4 <: bool
@@ -22,14 +26,23 @@ assume val mm256_shuffle_epi32_lemma (a:i32) (b:bv256) (i:u64{v i < 8}):
         [SMTPat (to_i32x8 (Libcrux_intrinsics.Avx2.mm256_shuffle_epi32 a b) i)]
 
 assume val mm256_sub_epi32_lemma (a b: bv256) (i:u64{v i < 8}):
-  Lemma (to_i32x8 (Libcrux_intrinsics.Avx2.mm256_sub_epi32 a b) i == 
+  Lemma (to_i32x8 (Libcrux_intrinsics.Avx2.mm256_sub_epi32 a b) i ==
          sub_mod (to_i32x8 a i) (to_i32x8 b i))
          [SMTPat (to_i32x8 (Libcrux_intrinsics.Avx2.mm256_sub_epi32 a b) i)]
 
 assume val mm256_add_epi32_lemma (a b: bv256) (i:u64{v i < 8}):
-  Lemma (to_i32x8 (Libcrux_intrinsics.Avx2.mm256_add_epi32 a b) i == 
+  Lemma (to_i32x8 (Libcrux_intrinsics.Avx2.mm256_add_epi32 a b) i ==
          add_mod (to_i32x8 a i) (to_i32x8 b i))
          [SMTPat (to_i32x8 (Libcrux_intrinsics.Avx2.mm256_add_epi32 a b) i)]
+
+assume val mm256_mul_epi32_lemma (a b: bv256) (i:u64{v i < 8}):
+  Lemma (to_i32x8 (Libcrux_intrinsics.Avx2.mm256_mul_epi32 a b) i ==
+         (
+           let j = i /! mk_int 2 in
+           let v64 = (cast (to_i32x8 a j) <: i64) *! (cast (to_i32x8 b j) <: i64) in
+           if v i % 2 = 0 then cast (v64 >>! mk_u64 4) else cast v64
+         ))
+         [SMTPat (to_i32x8 (Libcrux_intrinsics.Avx2.mm256_mul_epi32 a b) i)]
 
 assume val mm256_set_epi32_lemma (x0 x1 x2 x3 x4 x5 x6 x7:i32) (i:u64{v i < 8}):
   Lemma (to_i32x8 (Libcrux_intrinsics.Avx2.mm256_set_epi32 x0 x1 x2 x3 x4 x5 x6 x7) i ==
@@ -50,6 +63,54 @@ assume val mm256_set_epi32_lemma (x0 x1 x2 x3 x4 x5 x6 x7:i32) (i:u64{v i < 8}):
           <:
           i32))
   [SMTPat (to_i32x8 (Libcrux_intrinsics.Avx2.mm256_set_epi32 x0 x1 x2 x3 x4 x5 x6 x7) i)]
+
+assume val mm256_blend_epi32_lemma (imm8: i32) (a b: bv256) (i:u64{v i < 8}):
+  Lemma (to_i32x8 (Libcrux_intrinsics.Avx2.mm256_blend_epi32 imm8 a b) i ==
+        (if ((imm8 >>! i <: i32) %! mk_i32 2 <: i32) =. mk_i32 0 <: bool
+         then to_i32x8 a i
+         else to_i32x8 b i))
+
+assume val mm256_set_m128i_lemma (hi lo: bv128) (i:u64{v i < 8}):
+  Lemma (to_i32x8 (Libcrux_intrinsics.Avx2.mm256_set_m128i hi lo) i ==
+        (match i <: u64 with
+        | Rust_primitives.Integers.MkInt 0 -> to_i32x4 lo (mk_u64 0)
+        | Rust_primitives.Integers.MkInt 1 -> to_i32x4 lo (mk_u64 1)
+        | Rust_primitives.Integers.MkInt 2 -> to_i32x4 lo (mk_u64 2)
+        | Rust_primitives.Integers.MkInt 3 -> to_i32x4 lo (mk_u64 3)
+        | Rust_primitives.Integers.MkInt 4 -> to_i32x4 hi (mk_u64 0)
+        | Rust_primitives.Integers.MkInt 5 -> to_i32x4 hi (mk_u64 1)
+        | Rust_primitives.Integers.MkInt 6 -> to_i32x4 hi (mk_u64 2)
+        | Rust_primitives.Integers.MkInt 7 -> to_i32x4 hi (mk_u64 3)
+        | _ ->
+          Rust_primitives.Hax.never_to_any (Core.Panicking.panic "internal error: entered unreachable code"
+
+              <:
+              Rust_primitives.Hax.t_Never)
+          <:
+          i32))
+  [SMTPat (to_i32x8 (Libcrux_intrinsics.Avx2.mm256_set_m128i hi lo) i)]
+
+assume val mm256_permute2x128_si256_lemma_i32x4 (imm8: i32) (a b: bv256) (j:u64{v j < 8}):
+  Lemma (to_i32x8 (Libcrux_intrinsics.Avx2.mm256_permute2x128_si256 imm8 a b) j ==
+        (
+          let i:u64 = j /! mk_int 4 in
+          let offset = v j % 4 in
+          let control:i32 = imm8 >>! (i *! mk_u64 4 <: u64) in
+          if ((control >>! mk_i32 3 <: i32) %! mk_i32 2 <: i32) =. mk_i32 1
+          then mk_i32 0
+          else
+            match control %! mk_i32 4 <: i32 with
+            | Rust_primitives.Integers.MkInt 0 -> to_i32x8 a (mk_u64 (0 + offset))
+            | Rust_primitives.Integers.MkInt 1 -> to_i32x8 a (mk_u64 (4 + offset))
+            | Rust_primitives.Integers.MkInt 2 -> to_i32x8 b (mk_u64 (0 + offset))
+            | Rust_primitives.Integers.MkInt 3 -> to_i32x8 b (mk_u64 (4 + offset))
+            )
+        )
+  [SMTPat (to_i32x8 (Libcrux_intrinsics.Avx2.mm256_permute2x128_si256 imm8 a b) j)]
+
+assume val mm256_castsi256_si128_lemma (a: bv256) (i:u64{v i < 4}):
+  Lemma (to_i32x4 (Libcrux_intrinsics.Avx2.mm256_castsi256_si128 a) i == to_i32x8 a i)
+  [SMTPat (to_i32x4 (Libcrux_intrinsics.Avx2.mm256_castsi256_si128 a) i)]
 
 assume val mm256_unpacklo_epi64_lemma (a b: bv256) (i:u64{v i < 8}):
   Lemma (to_i32x8 (Libcrux_intrinsics.Avx2.mm256_unpacklo_epi64 a b) i ==
@@ -93,10 +154,34 @@ assume val mm256_unpackhi_epi64_lemma (a b: bv256) (i:u64{v i < 8}):
 
 assume val mont_mul: i32 -> i32 -> i32
 
-assume val montgomery_multiply_lemma 
+
+assume val montgomery_multiply_aux_lemma field_modulus inverse_of_modulus_mod_montgomery_r
+  (a b: Core_models.Abstractions.Bitvec.t_BitVec (mk_u64 256))
+  (i:u64{v i < 8}):
+  Lemma 
+    (requires
+        field_modulus ==
+        (Libcrux_intrinsics.Avx2.mm256_set1_epi32 Libcrux_ml_dsa.Simd.Traits.v_FIELD_MODULUS
+          <:
+          Core_models.Abstractions.Bitvec.t_BitVec (mk_u64 256)) /\
+        inverse_of_modulus_mod_montgomery_r ==
+        (Libcrux_intrinsics.Avx2.mm256_set1_epi32 (cast (Libcrux_ml_dsa.Simd.Traits.v_INVERSE_OF_MODULUS_MOD_MONTGOMERY_R
+                  <:
+                  u64)
+              <:
+              i32)
+          <:
+          Core_models.Abstractions.Bitvec.t_BitVec (mk_u64 256)))
+  (ensures
+    to_i32x8 (Libcrux_ml_dsa.Simd.Avx2.Arithmetic.montgomery_multiply_aux field_modulus inverse_of_modulus_mod_montgomery_r a b) i ==
+    mont_mul (to_i32x8 a i) (to_i32x8 b i))
+    [SMTPat (to_i32x8 (Libcrux_ml_dsa.Simd.Avx2.Arithmetic.montgomery_multiply_aux field_modulus inverse_of_modulus_mod_montgomery_r a b) i)]
+
+let montgomery_multiply_lemma
   (a b: Core_models.Abstractions.Bitvec.t_BitVec (mk_u64 256))
   (i:u64{v i < 8}):
   Lemma (
     to_i32x8 (Libcrux_ml_dsa.Simd.Avx2.Arithmetic.montgomery_multiply a b) i ==
     mont_mul (to_i32x8 a i) (to_i32x8 b i))
     [SMTPat (to_i32x8 (Libcrux_ml_dsa.Simd.Avx2.Arithmetic.montgomery_multiply a b) i)]
+   = ()
